CredibleCompilation/DCEOpt.lean
@@ -51,6 +51,7 @@ def transformInstr (prog : Prog) (revMap : Array Nat) (origPC : Nat) : TAC :=
   | some (.fbinop x op y z) => .fbinop x op y z
   | some (.intToFloat x y) => .intToFloat x y
   | some (.floatToInt x y) => .floatToInt x y
+  | some (.floatExp x y)   => .floatExp x y
   | some .halt             => .halt
   | some (.goto l)         => .goto (revMap.getD l 0)
   | some (.ifgoto b l)     => .ifgoto b (revMap.getD l 0)
@@ -79,7 +80,7 @@ def buildInstrCerts (origMap : Array Nat) (trans : Prog) : Array EInstrCert :=
       { pc_orig := origPC, transitions := ([] : List ETransCorr) }
     | some (.const _ _) | some (.copy _ _) | some (.binop _ _ _ _) | some (.boolop _ _)
     | some (.arrLoad _ _ _ _) | some (.arrStore _ _ _ _)
-    | some (.fbinop _ _ _ _) | some (.intToFloat _ _) | some (.floatToInt _ _) =>
+    | some (.fbinop _ _ _ _) | some (.intToFloat _ _) | some (.floatToInt _ _) | some (.floatExp _ _) =>
       let nextOrigPC := origMap.getD (i + 1) 0
       { pc_orig := origPC, transitions := [{ origLabels := (nextOrigPC :: []) }] }
     | some (.goto l) =>
