CredibleCompilation/RegAllocOpt.lean
@@ -206,6 +206,7 @@ def renameInstr (coloring : List (Var × String)) (instr : TAC) : TAC :=
   | .fbinop x op y z => .fbinop (r x) op (r y) (r z)
   | .intToFloat x y  => .intToFloat (r x) (r y)
   | .floatToInt x y  => .floatToInt (r x) (r y)
+  | .floatExp x y    => .floatExp (r x) (r y)
   | .goto l          => .goto l
   | .ifgoto be l     => .ifgoto (renameBoolExpr coloring be) l
   | .halt            => .halt
@@ -276,6 +277,7 @@ def renameProg (prog : Prog) (coloring : List (Var × String)) : Prog :=
     | .fbinop x _ _ _   => fun w => if w == x then .float else ctx w
     | .intToFloat x _   => fun w => if w == x then .float else ctx w
     | .floatToInt x _   => fun w => if w == x then .int else ctx w
+    | .floatExp x _     => fun w => if w == x then .float else ctx w
     | .arrLoad x _ _ ty => fun w => if w == x then ty else ctx w
     | _                  => ctx
   ) prog.tyCtx
