benchmarks/livermore/k22_planck.w
@@ -1,0 +1,23 @@
+var k : int, rep : int, expx : float, s : float;
+array x[1024] : float, y[1024] : float;
+
+k := 0;
+while (k < 1024) {
+  x[k] := intToFloat(k) * 0.01 + 0.01;
+  k := k + 1
+};
+
+s := 0.0;
+
+rep := 0;
+while (rep < 10000) {
+  k := 0;
+  while (k < 1024) {
+    expx := exp(x[k]);
+    y[k] := x[k] / (expx - 1.0);
+    k := k + 1
+  };
+  rep := rep + 1
+};
+
+s := y[0]
